examples/scache/CacheIO.i.dfy
@@ -1,0 +1,87 @@
+include "Cache.i.dfy"
+
+module CacheIOImpl {
+  import opened CacheImpl
+  import opened Constants
+  import opened Ptrs
+  import opened NativeTypes
+  import RWLock
+  import CacheResources
+  import LinearMaps
+  import opened DiskInterfaceSpec
+
+  method get_free_io_slot(c: Cache)
+  returns (idx: uint64, linear access: IOSlotAccess)
+  requires Inv(c)
+  ensures 0 <= idx as int < NUM_IO_SLOTS
+  ensures is_slot_access(c.io_slots[idx], access)
+
+  method disk_writeback_async(
+      c: Cache,
+      disk_idx: uint64,
+      cache_idx: uint64,
+      /*readonly*/ linear contents: Ptrs.ArrayDeref<byte>,
+      linear g: WritebackGhostState,
+      linear ticket: DiskWriteTicket)
+  requires Inv(c)
+  requires 0 <= cache_idx as int < CACHE_SIZE
+  requires 0 <= disk_idx as int < NUM_DISK_PAGES
+  requires contents.ptr == c.data[cache_idx]
+  requires |contents.s| == 4096
+  requires ticket == DiskWriteTicket(disk_idx * 4096, contents.s)
+  {
+    var idx;
+    linear var access;
+    idx, access := get_free_io_slot(c);
+    linear var IOSlotAccess(aiocb, info) := access;
+
+    ptr_write(c.io_slots[idx].aiocb_ptr,
+        inout aiocb,
+        aiocb_constructor(disk_idx * 4096, c.data[cache_idx], 4096));
+
+    ptr_write(c.io_slots[idx].info_ptr,
+        inout info,
+        IOSlotWrite(cache_idx));
+
+    var old_v, new_v;
+    linear var old_g;
+    old_v, new_v, old_g := async_write(
+        c.disk_interface,
+        c.io_slots[idx].aiocb_ptr,
+        aiocb,
+        contents,
+        ticket);
+    ///////////////////////////////////////////////////////////////////
+    linear var DIGhost(writeMap, readMap) := old_g;
+    writeMap := LinearMaps.add(writeMap, c.io_slots[idx].aiocb_ptr,
+        WritebackGhostStateWithSlot(info, g));
+    linear var new_g := DIGhost(writeMap, readMap);
+    ///////////////////////////////////////////////////////////////////
+    disk_interface_op_cleanup(c.disk_interface, new_v, new_g);
+    ///////////////////////////////////////////////////////////////////
+  }
+
+  method disk_read_sync(
+      addr: uint64,
+      ptr: Ptr,
+      inout linear contents: ArrayDeref<byte>,
+      linear ticket: DiskReadTicket)
+  returns (linear stub: DiskReadStub)
+  requires |old_contents.s| == 4096
+  requires ticket == DiskReadTicket(addr)
+  requires old_contents.ptr == ptr
+  ensures contents.ptr == ptr
+  ensures |contents.s| == 4096
+  ensures stub == DiskReadStub(addr, contents.s)
+
+
+  /*method disk_writeback_callback(
+      c: Cache,
+      addr: uint64,
+      /*readonly*/ linear contents: Ptrs.ArrayDeref<byte>,
+      linear g: CacheIOImpl.WritebackGhostState,
+      linear stub: CacheResources.R)
+  requires Inv(c)
+  requires stub == CacheResources.DiskWriteStub(addr)
+  requires g.WF(addr)*/
+}
